code/ecdsap256/Hacl.Impl.ECDSA.MontgomeryMultiplication.fsti
@@ -42,7 +42,8 @@ val reduction_prime_2prime_with_carry: #c: curve -> x: widefelem c -> result: fe
   Stack unit 
     (requires fun h -> live h x /\ live h result /\  eq_or_disjoint x result /\ wide_as_nat c h x < 2 * prime_p256_order)
     (ensures fun h0 _ h1 -> modifies (loc result) h0 h1 /\ as_nat c h1 result = wide_as_nat c h0 x % prime_p256_order)  
-    
+
+
 inline_for_extraction noextract
 val reduction_prime_2prime_with_carry2: #c: curve ->  carry: uint64 ->  x: felem c 
   -> result: felem c ->
